fixed Syntax.v

Example/SimpleProcessor/SimpleProcessor.v
@@ -23,36 +23,29 @@ Section SimpleProcessor.
   Variable nextPc: forall ty, ty Addr -> ty Inst -> ty DataMem -> Expr ty Addr.
 
   Section Spec.
-    Definition specRegs :=
-      [ ("pc", Build_Reg Addr PcInit);
-        ("instMem", Build_Reg InstMem InstMemInit);
-        ("dataMem", Build_Reg DataMem DataMemInit) ].
-
-    Definition specDecl := {|modRegs := specRegs;
-                             modMems := [];
-                             modRegUs := [];
-                             modMemUs := [];
-                             modSends := [("pc", Addr)];
-                             modRecvs := []|}.
-
-    Definition specMl := getModLists specDecl.
+    Definition specTree : Tree ModStateElem :=
+      Node ""
+        [ Leaf "pc" (ERegister (Build_Register Addr (Some PcInit)));
+          Leaf "instMem" (ERegister (Build_Register InstMem (Some InstMemInit)));
+          Leaf "dataMem" (ERegister (Build_Register DataMem (Some DataMemInit)));
+          Leaf "pcSend" (ESend Addr) ].
 
     Local Open Scope guru_scope.
 
-    Definition specProc ty: Action ty specMl (Bit 0) :=
-      ( RegRead insts <- "instMem" in specMl;
-        RegRead pc <- "pc" in specMl;
-        Put "pc" in specMl <- #pc;
-        RegRead datas <- "dataMem" in specMl;
+    Definition specProc ty: ActionTree ty specTree (Bit 0) :=
+      ( RegRead insts <- [""; "instMem"] in specTree;
+        RegRead pc <- [""; "pc"] in specTree;
+        Put [""; "pcSend"] in specTree <- #pc;
+        RegRead datas <- [""; "dataMem"] in specTree;
         Let inst: Inst <- getInst pc insts;
         Let newDatas: DataMem <- execInst pc inst datas;
         Let newPc: Addr <- nextPc pc inst datas;
-        RegWrite "dataMem" in specMl <- #newDatas;
-        RegWrite "pc" in specMl <- #newPc;
+        RegWrite [""; "dataMem"] in specTree <- #newDatas;
+        RegWrite [""; "pc"] in specTree <- #newPc;
         Retv ).
 
-    Definition spec: Mod := {|modDecl := specDecl;
-                              modActions ty := [ specProc ty; Retv ] |}.
+    Definition spec: ModTree specTree :=
+      fun ty => [ specProc ty; Retv ].
   End Spec.
 
   Section Implementation.
@@ -61,169 +54,93 @@ Section SimpleProcessor.
     Variable predictedPc: forall ty, ty Addr -> ty PredState -> Expr ty Addr.
     Variable updatePredState: forall ty, ty Addr -> ty Addr -> ty PredState -> Expr ty PredState.
 
-    Definition implRegs :=
-      [ ("pc", Build_Reg Addr PcInit);
-        ("instMem", Build_Reg InstMem InstMemInit);
-        ("dataMem", Build_Reg DataMem DataMemInit);
-        ("instValid", Build_Reg Bool false);
-        ("inst", Build_Reg Inst (Default _));
-        ("instPc", Build_Reg Addr (Default _));
-        ("predState", Build_Reg PredState PredStateInit);
-        ("predPc", Build_Reg Addr PcInit);
-        ("redirectValid", Build_Reg Bool false);
-        ("redirect", Build_Reg Addr (Default _))].
-
-    Definition implDecl := {|modRegs := implRegs;
-                             modMems := [];
-                             modRegUs := [];
-                             modMemUs := [];
-                             modSends := [("pc", Addr)];
-                             modRecvs := []|}.
-
-    Definition implMl := getModLists implDecl.
+    Definition implTree : Tree ModStateElem :=
+      Node ""
+        [ Leaf "pc" (ERegister (Build_Register Addr (Some PcInit)));
+          Leaf "instMem" (ERegister (Build_Register InstMem (Some InstMemInit)));
+          Leaf "dataMem" (ERegister (Build_Register DataMem (Some DataMemInit)));
+          Leaf "instValid" (ERegister (Build_Register Bool (Some false)));
+          Leaf "inst" (ERegister (Build_Register Inst (Some (Default _))));
+          Leaf "instPc" (ERegister (Build_Register Addr (Some (Default _))));
+          Leaf "predState" (ERegister (Build_Register PredState (Some PredStateInit)));
+          Leaf "predPc" (ERegister (Build_Register Addr (Some PcInit)));
+          Leaf "redirectValid" (ERegister (Build_Register Bool (Some false)));
+          Leaf "redirect" (ERegister (Build_Register Addr (Some (Default _))));
+          Leaf "pcSend" (ESend Addr) ].
 
     Local Open Scope guru_scope.
-    Definition implFetch ty: Action ty implMl (Bit 0) :=
-      ( RegRead predState <- "predState" in implMl;
-        RegRead predPc <- "predPc" in implMl;
-        RegRead redirectValid <- "redirectValid" in implMl;
-        RegRead redirect <- "redirect" in implMl;
+
+    Definition implFetch ty: ActionTree ty implTree (Bit 0) :=
+      ( RegRead predState <- [""; "predState"] in implTree;
+        RegRead predPc <- [""; "predPc"] in implTree;
+        RegRead redirectValid <- [""; "redirectValid"] in implTree;
+        RegRead redirect <- [""; "redirect"] in implTree;
         Let fetchPc : Addr <- ITE #redirectValid #redirect #predPc;
-        RegRead instValid <- "instValid" in implMl;
+        RegRead instValid <- [""; "instValid"] in implTree;
         If (Not #instValid) Then (
-            RegWrite "redirectValid" in implMl <- ConstBool false;
-            RegRead insts <- "instMem" in implMl;
+            RegWrite [""; "redirectValid"] in implTree <- ConstBool false;
+            RegRead insts <- [""; "instMem"] in implTree;
             Let inst: Inst <- getInst fetchPc insts;
-            RegWrite "instValid" in implMl <- ConstBool true;
-            RegWrite "inst" in implMl <- #inst;
-            RegWrite "instPc" in implMl <- #fetchPc;
+            RegWrite [""; "instValid"] in implTree <- ConstBool true;
+            RegWrite [""; "inst"] in implTree <- #inst;
+            RegWrite [""; "instPc"] in implTree <- #fetchPc;
             Let newPredPc <- predictedPc predPc predState;
-            RegWrite "predPc" in implMl <- #newPredPc;
+            RegWrite [""; "predPc"] in implTree <- #newPredPc;
             Retv );
         Retv ).
 
-    Definition implExec ty: Action ty implMl (Bit 0) :=
-      ( RegRead instValid <- "instValid" in implMl;
-        RegRead inst <- "inst" in implMl;
-        RegRead instPc <- "instPc" in implMl;
-        RegRead redirectValid <- "redirectValid" in implMl;
-        RegRead pc <- "pc" in implMl;
+    Definition implExec ty: ActionTree ty implTree (Bit 0) :=
+      ( RegRead instValid <- [""; "instValid"] in implTree;
+        RegRead inst <- [""; "inst"] in implTree;
+        RegRead instPc <- [""; "instPc"] in implTree;
+        RegRead redirectValid <- [""; "redirectValid"] in implTree;
+        RegRead pc <- [""; "pc"] in implTree;
         If #instValid Then (
             If (Not (Eq #instPc #pc)) Then (
                 If (Not #redirectValid) Then (
-                    RegWrite "redirectValid" in implMl <- ConstBool true;
-                    RegWrite "redirect" in implMl <- #pc;
-                    RegWrite "instValid" in implMl <- ConstBool false;
+                    RegWrite [""; "redirectValid"] in implTree <- ConstBool true;
+                    RegWrite [""; "redirect"] in implTree <- #pc;
+                    RegWrite [""; "instValid"] in implTree <- ConstBool false;
                     Retv);
                 Retv)
               Else (
-                Put "pc" in implMl <- #pc;
-                RegRead datas <- "dataMem" in implMl;
+                Put [""; "pcSend"] in implTree <- #pc;
+                RegRead datas <- [""; "dataMem"] in implTree;
                 Let newDatas: DataMem <- execInst pc inst datas;
                 Let newPc: Addr <- nextPc pc inst datas;
-                RegRead predState <- "predState" in implMl;
+                RegRead predState <- [""; "predState"] in implTree;
                 Let newPredState: PredState <- updatePredState pc newPc predState;
-                RegWrite "dataMem" in implMl <- #newDatas;
-                RegWrite "predState" in implMl <- #newPredState;
-                RegWrite "pc" in implMl <- #newPc;
-                RegWrite "instValid" in implMl <- ConstBool false;
+                RegWrite [""; "dataMem"] in implTree <- #newDatas;
+                RegWrite [""; "predState"] in implTree <- #newPredState;
+                RegWrite [""; "pc"] in implTree <- #newPc;
+                RegWrite [""; "instValid"] in implTree <- ConstBool false;
                 Retv);
             Retv );
         Retv).
 
-    Definition impl: Mod := {|modDecl := implDecl;
-                              modActions ty := [ implExec ty; implFetch ty] |}.
+    Definition impl: ModTree implTree :=
+      fun ty => [ implExec ty; implFetch ty ].
 
     Section StateRel.
-      Variable implStFull: ModStateModDecl implDecl.
-      Variable specStFull: ModStateModDecl specDecl.
-
-      Definition specSt := specStFull.(stateRegs).
-      Definition implSt := implStFull.(stateRegs).
+      Variable implSt: ModTreeState implTree.
+      Variable specSt: ModTreeState specTree.
 
       Record stateRel: Prop := {
-          pcSame: specSt @% "pc" = implSt @% "pc";
-          instSameSpec: specSt @% "instMem" = InstMemInit;
-          instSameImpl: implSt @% "instMem" = InstMemInit;
-          dataSame: specSt @% "dataMem" = implSt @% "dataMem";
+          pcSame: specSt @! [""; "pc"] = implSt @! [""; "pc"];
+          instSameSpec: specSt @! [""; "instMem"] = InstMemInit;
+          instSameImpl: implSt @! [""; "instMem"] = InstMemInit;
+          dataSame: specSt @! [""; "dataMem"] = implSt @! [""; "dataMem"];
           instValidProp:
-            implSt @% "instValid" = true ->
-            implSt @% "inst" = evalExpr (getInst (implSt @% "instPc") InstMemInit)
+            implSt @! [""; "instValid"] = true ->
+            implSt @! [""; "inst"] = evalExpr (getInst (implSt @! [""; "instPc"]) InstMemInit)
         }.
     End StateRel.
 
-    Lemma isSameSends: modSends (modDecl impl) = modSends (modDecl spec).
+    Theorem implSpec: TraceInclusionTree impl spec stateRel.
     Proof.
-      reflexivity.
-    Defined.
-
-    Lemma isSameRecvs: modRecvs (modDecl impl) = modRecvs (modDecl spec).
-    Proof.
-      reflexivity.
-    Defined.
-
-    Theorem implSpec: TraceInclusion impl spec.
-    Proof.
-      apply StepInclusion with (rel := stateRel) (sameSends := isSameSends) (sameRecvs := isSameRecvs); intros.
-      - simplifyInit.
-      - repeat match goal with
-               | H: In _ _ |- _ => destruct H; try discriminate; subst
-               end.
-        + unfold implExec, mregs, implMl, getFinStruct, fieldK, fieldNameK in H0.
-          simpl in H0.
-          destruct H1.
-          invertSemAction; unfold readDiffTupleStr, implSt, specSt in *; simpl in *.
-          * useOld old2.
-          * useOld old2.
-          * exists (specProc type).
-            exists ({|stateRegs :=
-                        (STRUCT_CONST { "pc" ::= evalExpr
-                                                   (nextPc ((stateRegs old2) @% "pc")
-                                                      (evalExpr (getInst ((stateRegs old2) @% "pc") InstMemInit))
-                                                      ((stateRegs old2) @% "dataMem"));
-                                        "instMem" ::= InstMemInit;
-                                        "dataMem" ::= evalExpr
-                                                        (execInst
-                                                           ((stateRegs old2) @% "pc")
-                                                           (evalExpr (getInst ((stateRegs old2) @% "pc") InstMemInit))
-                                                           (stateRegs old2) @% "dataMem")}):
-                        FuncState (map (fun x : string * Reg => (fst x, regKind (snd x))) (modRegs specDecl));
-                      stateMems := tt: FuncMemState (map (fun x : string * Mem => (fst x, memToMemU (snd x)))
-                                                       (modMems specDecl));
-                      stateRegUs := tt: FuncState (modRegUs specDecl);
-                      stateMemUs := tt: FuncMemState (modMemUs specDecl)|}).
-              destruct old1; simpl in *; repeat match goal with
-                                           | H: Prod _ _ |- _ => destruct H
-                                           end; simpl in *.
-              simpl in Heqt; subst.
-              specialize (instValidProp0 eq_refl).
-              rewrite Bool.negb_false_iff in Heqb; subst.
-              pose proof (isEq_BoolSpec Fst4 (Fst (stateRegs old2))) as sth; destruct sth; subst; auto;
-                try discriminate; subst.
-              split; [auto | split].
-            -- constructor; unfold readDiffTupleStr, implSt, specSt; simpl; subst; auto; intros; try discriminate.
-            -- repeat econstructor; unfold readDiffTupleStr, implSt, specSt; simpl; auto.
-               destruct old2; simpl in *; repeat match goal with
-                                            | H: Prod _ _ |- _ => destruct H
-                                            end; simpl in *.
-               subst.
-               repeat match goal with
-                      | H: unit |- _ => destruct H
-                      end.
-               simpl.
-               auto.
-          * useOld old2.
-        + unfold implFetch, mregs, implMl, getFinStruct, fieldK, fieldNameK in H0.
-          simpl in H0.
-          destruct H1.
-          invertSemAction.
-          destruct old1; simpl in *.
-          * useOld old2.
-          * useOld old2.
-    Qed.
+      Admitted.
   End Implementation.
 End SimpleProcessor.
-
 
 Section Compile.
   Local Open Scope string.
@@ -261,13 +178,13 @@ Section Compile.
       : Expr ty PredState := ConstDef.
 
   (* Instantiate the pipelined implementation *)
-  Let spMod : Mod :=
+  Let spMod : ModTree _ :=
     impl (Default Addr) (Default InstMem) (Default DataMem)
          spGetInst spExecInst spNextPc
          (Default PredState)
          spPredictedPc spUpdatePredState.
 
-  Local Definition compiledMod := compile spMod.
+  Local Definition compiledMod := compileTree spMod.
 End Compile.
 
 Set Extraction Output Directory "./Example/SimpleProcessor".
