Example/Test/Test.v
@@ -56,34 +56,32 @@ Section T.
   End Ty.
 
   Local Open Scope string.
-  Let decl := {|modRegs := [("r", Build_Reg Bool true) ];
-                (* modMems := [("m", @Build_Mem 3 Bool 5 None)]; *)
-                modMems := [("m", @Build_Mem 3 Bool 5
-                                    (Some (@Build_SameTuple _ 3 [true; true; false] I,
-                                         Build_VerilogMem true "" 0 0)))];
-                modRegUs := [("ru", Bool) ];
-                modMemUs := [("mu", Build_MemU 6 Bool 3)];
-                modSends := [("p", Bool)];
-                modRecvs := [("g", Bool)]|}.
 
-  Let ml := getModLists decl.
+  Definition testTree : Tree ModStateElem :=
+    Node ""
+      [ Leaf "r" (ERegister (Build_Register Bool (Some true)));
+        Leaf "m" (EMemory (Build_Memory 3 Bool 5 (Some (Some (@Build_SameTuple _ 3 [true; true; false] I)))));
+        Leaf "ru" (ERegister (Build_Register Bool (Some (Default Bool))));
+        Leaf "mu" (EMemory (Build_Memory 6 Bool 3 None));
+        Leaf "p" (ESend Bool);
+        Leaf "g" (ERecv Bool) ].
 
   Local Set Printing Depth 1000.
-  Let act ty: Action ty ml Bool := structSimplCbn
-        ( RegRead tr <- "r" in ml;
-          RegWrite "r" in ml <- ConstBool true;
-          MemReadRq "m" in ml !1 <- ConstDef;
-          MemReadRp tm <- "m" in ml !4;
-          MemWrite "m" in ml ! ConstBit (Zmod.of_Z _ (-1)) <- #tm;
-          RegReadU tru <- "ru" in ml;
-          RegWriteU "ru" in ml <- Not #tru;
-          MemReadRqU "mu" in ml !1 <- Add [ConstBit (Zmod.of_Z _ 4); ConstBit (Zmod.of_Z _ 0xf);
+  Let act ty: ActionTree ty testTree Bool := structSimplCbn
+        ( RegRead tr <- "r" in testTree;
+          RegWrite "r" in testTree <- ConstBool true;
+          MemReadRq "m" in testTree !1 <- ConstDef;
+          MemReadRp tm <- "m" in testTree !4;
+          MemWrite "m" in testTree ! ConstBit (Zmod.of_Z _ (-1)) <- #tm;
+          RegRead tru <- "ru" in testTree;
+          RegWrite "ru" in testTree <- Not #tru;
+          MemReadRq "mu" in testTree !1 <- Add [ConstBit (Zmod.of_Z _ 4); ConstBit (Zmod.of_Z _ 0xf);
                                            ConstBit (Zmod.of_Z _ 0xe);
                                            ConstBit (Zmod.of_Z _ 2); ConstBit (Zmod.of_Z _ 1)];
-          MemReadRpU tmu <- "mu" in ml !0;
-          MemWriteU "mu" in ml ! ConstBit (Zmod.of_Z _ 3) <- #tmu;
-          Put "p" in ml <- ConstDefK Bool;
-          Get tg <- "g" in ml;
+          MemReadRp tmu <- "mu" in testTree !0;
+          MemWrite "mu" in testTree ! ConstBit (Zmod.of_Z _ 3) <- #tmu;
+          Put "p" in testTree <- ConstDefK Bool;
+          Get tg <- "g" in testTree;
           Random tv7: Bit 6 ;
           Let structVal: STRUCT_TYPE {"a" :: Bool ; "b" :: Bit 2} <- STRUCT { "a" ::= Const ty Bool false;
                                                                               "b" ::= Const ty (Bit _)
@@ -95,78 +93,54 @@ Section T.
           Let var : Bit 4 <- $4;
           Let var2 : Bit 2 <- #var`[1:0];
           LetA tv3 : Bit 4 <- ( Let tv4: Bit 4 <- ZeroExtend 2 (Concat (ToBit #tv) (ToBit #tg));
-                                Return #tv4);
+                                ReturnTree #tv4);
           LetA tv6 <- ( Let tv5 <- (Concat (ToBit #tv) (ToBit #tg));
-                        Return #tv5);
-          
-          LetL test: Bool <- ( SysE [];
-                               LetE l1 <- #tr;
-                               LetE l2 : Bool <- Not #l1;
-                               LETE l22 : Bool <- (RetE #l2);
-                               LetIfE l3: Bool <- IfE #l1 ThenE (RetE #l2) ElseE (RetE (Not #l2)) ;
-                               LetIfE l4 <- IfE #l2 ThenE (RetE #l1) ElseE (RetE (Not #l1));
-                               RetE #l4);
+                        ReturnTree #tv5);
           
           Let structVal : S1 <- s1 ty;
           Let newTr <- #structVal`"test";
-          
-          LetL tes1 <- ( SysE [];
-                         LetE l1 <- #newTr;
-                         LetE l2 : Bool <- Not #l1;
-                         LetIfE l3: Bool <- IfE #l1 ThenE (RetE #l2) ElseE (RetE (Not #l2)) ;
-                         LetIfE l4 <- IfE #l2 ThenE (RetE #l1) ElseE (RetE (Not #l1));
-                         RetE #l4);
           
           LetIf foo1: Bit 1 <-
                         If #tg Then (
                           LetIf bar1 : Bool <-
                                          If #tv Then (
-                                           Return (Not #tg)
+                                           ReturnTree (Not #tg)
                                          ) Else (
-                                           Return ConstDef
+                                           ReturnTree ConstDef
                                          );
-                          Return (ToBit #tr)
+                          ReturnTree (ToBit #tr)
                         ) Else (
                           If (FromBit Bool (TruncLsb 5 1 #tv7)) Then (
                               Sys [];
-                              Return (ConstDefK (Bit 4))
+                              ReturnTree (ConstDefK (Bit 4))
                             );
-                          Return (ToBit #tm) ) ;
+                          ReturnTree (ToBit #tm) ) ;
           LetIf foo2 <-
             If #tg Then (
-              Return #tr
+              ReturnTree #tr
             ) Else (
-              Return #tm ) ;
+              ReturnTree #tm ) ;
           LetIf foo3: Bool <-
                         If #tg Then (
-                          Return #tr ) ;
+                          ReturnTree #tr ) ;
           LetIf foo4 <-
             If #tg Then (
-              Return #tr ) ;
+              ReturnTree #tr ) ;
           If #tg Then (
-              Return #tr
+              ReturnTree #tr
             ) Else (
-              Return (Not #tr)) ;
+              ReturnTree (Not #tr)) ;
           If #tg Then (
-              Return #tr );
+              ReturnTree #tr );
           Sys [];
-          Return (And [#tr;
-                       #tm;
-                       #tg]) ).
+          ReturnTree (And [#tr;
+                           #tm;
+                           #tg]) ).
 
-  Let listIntentationNotBroken := [ 5;
-                                    6 ; 8 ;
-                                    9].
+  Let m: ModTree testTree :=
+    fun ty => [ Act (act ty); ReturnTree ConstDef ].
 
-  Let listIntentationNotBroken2 := [
-      5;
-      6 ; 8 ;
-      9].
-
-  Let m: Mod := {|modDecl := decl;
-                  modActions := fun ty => [ Act (act ty); Return ConstDef ] |}.
-
-  Local Definition compiledMod := compile m.  
+  Local Definition compiledMod := compileTree m.  
 End T.
 
 Set Extraction Output Directory "./Example/Test".
